Use head instead of headOrFalse in normalization tests #183

base/coq/Free/Verification/NormalizationTests.v
@@ -42,6 +42,11 @@ Definition evalTracingNF {A B : Type}
                          `{Normalform _ _ A B} p
   := evalTracing (nf p).
 
+(* Handle a traced program after normalization. *)
+Definition evalTracingMaybeNF {A B : Type} 
+                         `{Normalform _ _ A B} p
+  := evalTracing (runMaybe (nf p)).
+
 (* Handle a possibly partial program after normalization. *)
 Definition evalMaybeNF {A B : Type} 
                        `{Normalform _ _ A B} p
@@ -161,15 +166,6 @@ Section SecData.
                             (Nil Shape Pos)))
         (Nil Shape Pos).
 
-  (* A function that is the same as head for non-empty lists.
-     Empty lists yield false. *)
-  Definition headOrFalse (fl : FreeBoolList)
-    : Free Shape Pos bool
-   := fl >>= fun l => match l with
-      | List.nil => pure false
-      | List.cons fb _ => fb
-      end.
-
 End SecData.
 
 (* Arguments sentences for the effectful lists. *)
@@ -183,7 +179,6 @@ Arguments tracedTraceList {_} {_} {_}.
 Arguments NDCoinList {_} {_} {_}.
 Arguments deepCoinList {_} {_} {_}.
 Arguments deepTraceList {_} {_} {_}.
-Arguments headOrFalse {_} {_} fl. 
 
 (* Section for auxiliary properties *)
 Section SecProps.
@@ -305,31 +300,31 @@ Proof. constructor. Qed.
 (* Normalization combined with non-strictness. *)
 
 (* Non-strictness should be preserved, so no tracing should occur.
-   headOrFalse [true, trace "component effect" false] --> (true,[]) *)
-Example nonStrictnessNoTracing : evalTracingNF (headOrFalse traceList)
- = (true, []).
+   headList _ _ MaybePartial [true, trace "component effect" false] --> (true,[]) *)
+Example nonStrictnessNoTracing : evalTracingMaybeNF (headList _ _ MaybePartial traceList)
+ = (Some true, []).
 Proof. constructor. Qed.
 
 (* Non-strictness should be preserved, so no non-determinism should occur.
-   headOrFalse [true,coin] --> [true] *)
-Example nonStrictnessNoND : evalNDNF (headOrFalse coinList)
- = [true].
+   head [true,coin] --> [true] *)
+Example nonStrictnessNoND : evalNDMaybeNF (headList _ _ MaybePartial coinList)
+ = [Some true].
 Proof. constructor. Qed.
 
 (* Evaluating the defined part of a partial list is still possible.
-   headOrFalse [true,undefined] --> true *)
+   head [true,undefined] --> true *)
 (* Since Maybe is still handled, the actual result should be Some true. *)
 Example nonStrictnessPartiality : evalMaybeNF 
-                                    (headOrFalse 
+                                    (headList _ _ MaybePartial 
                                       (partialList MaybePartial))
  = Some true.
 Proof. constructor. Qed.
 
-(* headOrFalse [true, false ? undefined] --> true *)
+(* headList _ _ MaybePartial [true, false ? undefined] --> true *)
 (* Since non-determinism and Maybe are still handled, the actual 
    result should be [Some true]. *)
 Example nonStrictnessNDPartiality : evalNDMaybeNF 
-                                    (headOrFalse 
+                                    (headList _ _ MaybePartial 
                                       (partialCoinList MaybePartial))
  = [Some true].
 Proof. constructor. Qed.
@@ -354,20 +349,20 @@ Proof. constructor. Qed.
 (* Combining non-strictness with effects at different levels. *)
 
 (* Only the message at the root should be logged. 
-   headOrFalse (trace "root effect" [true, trace "component effect" false])
+   headList _ _ MaybePartial (trace "root effect" [true, trace "component effect" false])
    --> (true, ["root effect") *)
 Example nonStrictnessRootAndComponentTracing 
- : evalTracing (headOrFalse tracedTraceList)
- = (true, ["root effect"%string]).
+ : evalTracingMaybeNF (headList _ _ MaybePartial tracedTraceList)
+ = (Some true, ["root effect"%string]).
 Proof. constructor. Qed.
 
 (* Only the choice at the root should be triggered. 
    Because the first list is empty and the second has true as its 
    first element, the results should be false and true.
-   headOrFalse ([] ? [true, coin]) --> [false,true] *)
+   head ([] ? [true, coin]) --> [undefined,true] *)
 Example nonStrictnessRootAndComponentND 
- : evalNDNF (headOrFalse NDCoinList) 
- = [false;true].
+ : evalNDMaybeNF (headList _ _ MaybePartial NDCoinList) 
+ = [None; Some true].
 Proof. constructor. Qed.
 
 (* Normalization of lists with effects nested deeper inside. *)
